semantics/cceval2.v
@@ -1,0 +1,158 @@
+Set Warnings "-notation-overridden,-parsing".
+From Coq Require Import Bool.Bool Init.Nat Arith.Arith Arith.EqNat
+     Init.Datatypes Lists.List Strings.String Program.
+Require Export Coq.Strings.String.
+From mathcomp Require Import ssreflect ssrfun ssrbool eqtype.
+Import ListNotations.
+From Semantics Require Import semantics.
+(*basic list functions that I couldn't find in a library*)
+Open Scope list_scope.
+Open Scope type_scope.
+
+(*written, read, written before reading*)
+Notation the_write_stuff := ((list loc) * (list loc) * (list loc)).
+
+(*Single steps, accumulates write data*)
+(*warning: OLD version below, most updated one in semantics*)
+Inductive cceval_w: context -> obseq -> context -> the_write_stuff -> Prop :=
+CheckPoint: forall(N: nvmem)
+               (V: vmem)
+               (c: command)
+               (w: warvars),
+    cceval_w (N, V, ((incheckpoint w);; c))
+             [checkpoint]
+             (N, V, c)
+             (nil, nil, nil)
+| NV_Assign: forall(x: smallvar) (N: nvmem) (V: vmem) (e: exp) (r: readobs) (v: value),
+    eeval N V e r v ->
+    isNV(x) -> (*checks x is correct type for NV memory*)
+    (isvaluable v) -> (*extra premise to check if v is valuable*)
+    cceval_w (N, V, Ins (asgn_sv x e))
+             [Obs r]
+             ((updateNV N (inl x) v), V, Ins skip)
+             ([inl x],  (readobs_loc r), (remove in_loc_b (readobs_loc r) [inl x]))
+| V_Assign: forall(x: smallvar) (N: nvmem) (mapV: mem) (e: exp) (r: readobs) (v: value),
+    eeval N (Vol mapV) e r v ->
+    isV(x) -> (*checks x is correct type for V memory*)
+    (isvaluable v) -> (*extra premise to check if v is valuable*)
+    cceval_w (N, (Vol mapV), Ins (asgn_sv x e)) [Obs r]
+             (N, (Vol ((inl x) |-> v ; mapV)), Ins skip)
+             (nil,  (readobs_loc r), nil)
+| Assign_Arr: forall (N: nvmem) (V: vmem)
+               (a: array)
+               (ei: exp)
+               (ri: readobs)
+               (vi: value)
+               (e: exp)
+               (r: readobs)
+               (v: value)
+               (element: el),
+    eeval N V ei ri vi ->
+    eeval N V e r v ->
+    (el_arrayind_eq element a vi) -> (*extra premise to check that inr element
+                                        is actually a[vindex] *)
+(*well-typedness, valuability, inboundedness of vindex are checked in elpred*)
+    (isvaluable v) -> (*extra premise to check if v is valuable*)
+    cceval_w (N, V, Ins (asgn_arr a ei e))
+           [Obs (ri++r)]
+           ((updateNV N (inr element) v), V, Ins skip)
+           ([inr element], (readobs_loc (ri ++ r)), (remove in_loc_b (readobs_loc (ri ++ r)) [inr element]))
+(*valuability and inboundedness of vindex are checked in sameindex*)
+| Skip: forall(N: nvmem)
+         (V: vmem)
+         (c: command),
+    cceval_w (N, V, (skip;;c)) [Obs NoObs] (N, V, c) (nil, nil, nil)
+| Seq: forall (N N': nvmem)
+         (V V': vmem)
+         (l: instruction)
+         (c: command)
+         (o: obs)
+         (WT1 RD1 FstWt1: list loc),
+    cceval_w (N, V, Ins l) [o] (N', V', Ins skip) (WT1, RD1, FstWt1) ->
+    cceval_w (N, V, (l;;c)) [o] (N', V', c) (WT1, RD1, FstWt1)
+| If_T: forall(N: nvmem)
+         (V: vmem)
+         (e: exp)
+         (r: readobs)
+         (c1 c2: command),
+    eeval N V e r true -> (*yuh doy not writing anything in eeval*)
+    cceval_w (N, V, (TEST e THEN c1 ELSE c2)) [Obs r] (N, V, c1) (nil, (readobs_loc r), nil)
+| If_F: forall(N: nvmem)
+         (V: vmem)
+         (e: exp)
+         (r: readobs)
+         (c1 c2: command),
+    eeval N V e r false ->
+    cceval_w (N, V, (TEST e THEN c1 ELSE c2)) [Obs r] (N, V, c2) (nil, (readobs_loc r), nil).
+
+(*Inductive iceval: iconf -> obseq -> iconf -> Prop :=
+  CP_PowerFail: forall(k: context) (N: nvmem) (V: vmem) (c: command),
+                 iceval (k, N, V, c)
+                        nil
+                        (k, N, (reset V), Ins inreboot)
+ | CP_CheckPoint: forall(k: context) (N: nvmem) (V: vmem) (c: command) (w: warvars),
+                 iceval (k, N, V, ((incheckpoint w);;c))
+                        [checkpoint]
+                        (((N |! w), V, c), N, V, c) 
+ | CP_Reboot: forall(N N': nvmem) (*see below*) (*N is the checkpointed one*)
+               (V V': vmem) 
+               (c: command), 
+     iceval ((N, V, c), N', V', Ins inreboot)
+            [reboot]
+            ((N, V, c), (N U! N'), V, c)
+ | CP_NV_Assign: forall(k: context) (x: smallvar) (N: nvmem) (V: vmem) (e: exp) (r: readobs) (v: value),
+    eeval N V e r v ->
+    isNV(x) -> (*checks x is correct type for NV memory*)
+    (isvaluable v) -> (*extra premise to check if v is valuable*)
+    iceval (k, N, V, Ins (asgn_sv x e))
+           [Obs r]
+           (k, (updateNV N (inl x) v), V, Ins skip)
+| CP_V_Assign: forall(k: context) (x: smallvar) (N: nvmem) (mapV: mem) (e: exp) (r: readobs) (v: value),
+    eeval N (Vol mapV) e r v ->
+    isV(x) -> (*checks x is correct type for V memory*)
+    (isvaluable v) -> (*extra premise to check if v is valuable*)
+    iceval (k, N, (Vol mapV), Ins (asgn_sv x e))
+           [Obs r]
+           (k, N, (Vol ((inl x) |-> v ; mapV)), Ins skip)
+| CP_Assign_Arr: forall (k: context) (N: nvmem) (V: vmem)
+               (a: array)
+               (ei: exp)
+               (ri: readobs)
+               (vi: value)
+               (e: exp)
+               (r: readobs)
+               (v: value)
+               (element: el),
+    eeval N V ei ri vi ->
+    eeval N V e r v ->
+    (el_arrayind_eq element a vi) -> (*extra premise to check that inr element
+                                        is actually a[vindex] *)
+(*well-typedness, valuability, inboundedness of vindex are checked in elpred*)
+    (isvaluable v) -> (*extra premise to check if v is valuable*)
+    iceval (k, N, V, Ins (asgn_arr a ei e))
+           [Obs (ri++r)]
+           (k, (updateNV N (inr element) v), V, Ins skip)
+| CP_Skip: forall(k: context) (N: nvmem)
+         (V: vmem)
+         (c: command),
+    iceval (k, N, V, (skip;;c)) [Obs NoObs] (k, N, V, c)
+|CP_Seq: forall (k: context)
+         (N: nvmem) (N': nvmem)
+         (V: vmem) (V': vmem)
+         (l: instruction)
+         (c: command)
+         (o: obs),
+    iceval (k, N, V, Ins l) [o] (k, N', V', Ins skip) ->
+    iceval (k, N, V, (l;;c)) [o] (k, N', V', c)
+|CP_If_T: forall(k: context) (N: nvmem) (V: vmem)
+         (e: exp)
+         (r: readobs)
+         (c1 c2: command),
+    eeval N V e r true -> 
+    iceval (k, N, V, (TEST e THEN c1 ELSE c2)) [Obs r] (k, N, V, c1)
+|CP_If_F: forall(k: context) (N: nvmem) (V: vmem)
+         (e: exp)
+         (r: readobs)
+         (c1 c2: command),
+    eeval N V e r false ->
+    iceval (k, N, V, (TEST e THEN c1 ELSE c2)) [Obs r] (k, N, V, c2).*)
