semantics/lemmas_0.v
@@ -1,0 +1,37 @@
+From Coq Require Import Bool.Bool Init.Nat Arith.Arith Arith.EqNat
+     Init.Datatypes Lists.List Strings.String Program.
+Require Export Coq.Strings.String.
+From mathcomp Require Import ssrnat ssreflect ssrfun ssrbool eqtype.
+From TLC Require Import LibTactics.
+
+Ltac destruct4r H L1 L2 L3 L4 := destruct H as [L1 rest];
+         destruct rest as [L2 rest];
+         destruct rest as [L3 L4].
+
+(*p sure this can actually be handled with case from ssreflect*)
+Ltac destruct3 Cmid nmid vmid cmid:=
+           destruct Cmid as [Annoying cmid]; destruct Annoying as [nmid vmid].
+
+Ltac ex_destruct3 H := destruct H as [var1 Annoying]; destruct Annoying as [var2 Annoying1];
+                       destruct Annoying1 as [var3 H].
+
+Ltac destruct_ms M T WT := destruct M as [WT neverseen]; destruct neverseen as [T].
+
+Ltac generalize_5 N N' V V' O := generalize dependent N;
+                               generalize dependent N';
+                               generalize dependent V;
+                               generalize dependent V';
+                               generalize dependent O.
+Ltac appldis applier appliee := apply applier in appliee; destruct appliee.
+
+Lemma reflect_conj: forall{b0 b1: bool} {P0 P1: Prop},
+                      reflect P0 b0 ->
+                      reflect P1 b1 ->
+                      reflect (P0 /\ P1) (b0 && b1).
+Proof. intros. case (b0 && b1) eqn: beq; constructor.
+       + appldis andb_true_iff beq. apply (elimT H) in H1.
+         apply (elimT H0) in H2. split; assumption.
+       + appldis andb_false_iff beq; case => contra1 contra2.
+         applys (elimF H) H1 contra1.
+         applys (elimF H0) H1 contra2.
+Qed.
