semantics/programs_error1.v
@@ -1,0 +1,259 @@
+Set Warnings "-notation-overridden,-parsing".
+From Coq Require Import Bool.Bool Init.Nat Arith.Arith Arith.EqNat
+     Init.Datatypes Strings.String Program Init.Logic.
+Require Export Coq.Strings.String.
+From mathcomp Require Import ssreflect ssrfun ssrbool eqtype seq ssrnat.
+From Semantics Require Import algorithms lemmas_1.
+
+
+Open Scope type_scope.
+(************* program traces*****************)
+
+(*trace helpers*)
+
+(*Notes:*)
+(*do I keep track of volatile writes as well...I don't think so
+ cuz the writes don't last and they all have to be checkpointed anyways*)
+(*concern:*)
+(*actually there's no reason for us to be checkpointing volatiles that are
+ written to before they're ever read from along any path*)
+(*at first inspection it doesn't seem like it would be all that hard to keep track of this
+ since we're already doing MFstWt for novolatiles.*)
+
+(*concern: cconf and context are functionally the same but cconf has an annoying constructor
+ which can't be coerced bc context exists, consider combining into one type?*)
+
+(*The trace type contains
+1. starting configuration
+2. ending configuration
+3. execution observations
+4. a list of warvars which have been written to
+5. a list of warvars which have been read from
+6. a list of warvars which have been written to before they have been read from
+ *)
+(*Ordering: start -> end -> observations -> the_write_stuff*)
+(*steps to termination, accumulates write data*)
+
+(*continuous traces*)
+
+Inductive trace_c: context -> context -> obseq -> the_write_stuff -> Type :=
+  CTrace_Empty: forall(C: context),
+                 trace_c C C [::] ([::], [::], [::])
+  | CTrace_Single: forall {C1 C2: context} {O: obseq} {W: the_write_stuff},
+      cceval_w C1 O C2 W ->
+      trace_c C1 C2 O W
+| CTrace_App: forall{C1 C2 Cmid: context} {O1 O2: obseq}
+               {W1 W2: the_write_stuff},
+    trace_c C1 Cmid O1 W1 -> (*steps first section*)
+    O1 <> [::] -> (* forces empty step to use other constructors*)
+    O2 <> [::]  ->
+    trace_c Cmid C2 O2 W2 -> (*steps rest of program*)
+    trace_c C1 C2 (O1 ++ O2) (append_write W1 W2).
+(*App makes for easy subtraces by allowing command in C2 not to be skip*)
+(*never actually need to append traces now that I have the write datatype
+ consider a simpler type?*)
+
+Print trace_c_ind.
+
+(*Theorem trace_c_ind_flex: forall
+         P : context ->
+             context ->
+             obseq ->
+             the_write_stuff -> Prop,
+       (forall C : context,
+        P C C [::] ([::], [::], [::])) ->
+       (forall (C1 C2 : context)
+          (O : obseq)
+          (W : the_write_stuff),
+        cceval_w C1 O C2 W -> P C1 C2 O W) ->
+       (forall (C1 C2 : context)
+          (O1 O2 : obseq)
+          (W1 W2 : the_write_stuff),
+      (exists(Cmid: context), trace_c C1 Cmid O1 W1 /\
+        P C1 Cmid O1 W1 /\ trace_c Cmid C2 O2 W2 /\
+        P Cmid C2 O2 W2) ->
+        O1 <> [::] ->
+        O2 <> [::] ->
+        P C1 C2 (O1 ++ O2)
+          (append_write W1 W2)) ->
+       forall (p p0 : context) 
+         (l : obseq)
+         (p1 : the_write_stuff),
+         trace_c p p0 l p1 -> P p p0 l p1.
+  Admitted.*)
+
+
+
+(*if you need the empty cat thing come back here*)
+Lemma empty_trace: forall{C1 C2: context} {O: obseq} {W: the_write_stuff},
+    trace_c C1 C2 O W -> O = [::] -> C1 = C2 /\ W = emptysets.
+Proof. intros. inversion X; subst.
+       + split; reflexivity.
+       + inversion H0.
+       + 
+         exfalso.
+ move / nilP : H4 => H4.
+         unfold nilp in H4.
+         apply (elimT eqP) in H4.
+         rewrite (size_cat O1 O2) in H4.
+         move / eqP : H4.
+         rewrite addn_eq0.
+         apply / andb_true_iff => H.
+         destruct H.
+           by move / nilP / H0 : H.
+Qed.
+
+Lemma append_write_empty: forall{W: the_write_stuff},
+    append_write W emptysets = W.
+Proof. intros. simpl. unfold append_write. simpl.
+       repeat rewrite cats0.
+       apply undo_gets.
+Qed.
+
+
+Lemma append_write_empty_l: forall{W: the_write_stuff},
+    append_write emptysets W = W.
+Proof. intros. simpl. unfold append_write. simpl.
+       unfold remove. simpl.
+       rewrite filter_predT. 
+       apply undo_gets.
+Qed.
+
+Program Definition trace_append {C1 Cmid C2: context }
+                  {O1 O2: obseq}
+                  {W1 W2: the_write_stuff}
+                  (T1: trace_c C1 Cmid O1 W1)
+                  (T2: trace_c Cmid C2 O2 W2) : trace_c C1 C2 (O1 ++ O2) (append_write W1 W2)
+  :=
+  match O1, O2 with
+    [::], [::] => T1 (*C1 = Cmid = C2*)
+  | [::], _ => T2 (*C1 = Cmid*)
+  | _, [::] => T1 (**)
+  | (x::xs), (y::ys) => CTrace_App T1 _ _ T2 end.
+
+(*clean up this ltac*)
+Ltac empty T2 :=apply empty_trace in T2; [destruct T2 as [f g ]; inversion f; subst; try reflexivity |
+                                           reflexivity].
+Ltac empty2 T1 T2 := apply empty_trace in T1; [destruct T1 as [f g]; inversion g;                 subst; apply empty_trace in T2; [ destruct T2 as [h i]; inversion i;
+                 rewrite append_write_empty; reflexivity | reflexivity] | reflexivity].
+
+Ltac emptyl T2 :=apply empty_trace in T2; [destruct T2 as [f g ]; inversion g; subst; try reflexivity |
+                                           reflexivity].
+
+Next Obligation. empty T2. Qed. 
+Next Obligation. empty2 T1 T2. Qed.           
+Next Obligation. empty T1. Qed.
+Next Obligation. emptyl T1. rewrite append_write_empty_l. reflexivity. Qed. 
+Next Obligation. empty T2. Qed.
+Next Obligation. by rewrite cats0. Qed.
+Next Obligation. emptyl T2. rewrite append_write_empty. reflexivity. Qed.
+Next Obligation. split. intros wildcard contra. destruct contra. inversion H1.
+                 intros contra. destruct contra. inversion H1. Qed.
+
+(*intermittent traces*)
+ (*the same as trace_c bar types as differences between
+  intermittent and continuous execution have been implemented in evals*)
+Inductive trace_i : iconf -> iconf -> obseq -> the_write_stuff -> Type :=
+iTrace_Empty: forall{C: iconf},
+                 trace_i C C [::] ([::], [::], [::])
+|iTrace_Single: forall{C1 C2: iconf} {O: obseq} {W: the_write_stuff},
+                  iceval_w C1 O C2 W -> (*command in C2 is skip by def single_com, iceval_w*)
+                  trace_i C1 C2 O W
+| iTrace_App: forall{C1 C2 Cmid: iconf} {O1 O2: obseq}
+         {W1 W2: the_write_stuff},
+    trace_i C1 Cmid O1 W1 -> (*steps first section*)
+    trace_i Cmid C2 O2 W2 -> (*steps rest of program*)
+    O1 <> [::] -> (* forces empty step to use other constructors*)
+    O2 <> [::]  ->
+    trace_i C1 C2 (O1 ++ O2) (append_write W1 W2).
+
+Definition multi_step_c (C1 C2: context) (O: obseq) :=
+    exists W: the_write_stuff, inhabited (trace_c C1 C2 O W).
+          
+
+Definition multi_step_i (C1 C2: iconf) (O: obseq) :=
+    exists W: the_write_stuff, inhabited (trace_i C1 C2 O W).
+(*more trace helpers*)
+
+Definition Wt {C1 C2: context} {O: obseq} {W: the_write_stuff}
+  (T: trace_c C1 C2 O W) := getwt W.
+
+Definition Rd {C1 C2: context} {O: obseq} {W: the_write_stuff}
+           (T: trace_c C1 C2 O W) := getrd W.
+
+Definition FstWt {C1 C2: context} {O: obseq} {W: the_write_stuff}
+  (T: trace_c C1 C2 O W) := getfstwt W.
+
+
+(**********************************************************************************)
+
+
+(*relations between continuous and intermittent memory*)
+
+
+(*Definition 4*)
+(*concern: not yet clear to me why we need the vmem parameter; pending further inspection of
+ proofs*)
+(*concern: liberal use of intensional equality with nvmem*)
+(*N0, V0 is starting state for both executions
+ N1, V1 and Ncomp are middle states of intermittent, continuous respectively
+ V1 isn't used anywhere it's just to fill out the type
+ N2, V2 is final state for intermittent, once again solely to fill out the type*)
+
+Inductive same_pt: nvmem -> vmem -> command -> command -> nvmem -> nvmem -> Prop:=
+same_mem: forall {N0 N1 Ncomp N2: nvmem}
+                  {V0 V1 V2: vmem}
+                  {c0 c1 crem: command}
+                  {W1 W2: the_write_stuff}
+                  {O1 O2: obseq}
+                  (T1: trace_c (N0, V0, c0) (N1, V1, c1) O1 W1)
+                  (T2: trace_c (N1, V1, c1) (N2, V2, crem) O2 W2),
+    crem = skip \/ (exists(w: warvars) (crem2: command), crem = ((incheckpoint w);;crem2)) ->
+                  subseq (getdomain Ncomp) (getdomain Ncomp) 
+                  -> not(checkpoint \in O1)
+                  -> not (checkpoint \in O2) (*checks checkpoint T2 ends on is nearest checkpoint*)
+                 -> (forall(l: loc),
+                      not((getmap N1) l = (getmap Ncomp) l)
+                      -> ((l \in (getwt W2)) /\ (l \in (getfstwt (append_write W1 W2))) /\ not (l \in (getwt W1))))
+                  -> same_pt N0 V0 c0 c1 N1 Ncomp.
+(*Definition 5*)
+(*Nc0 is starting nvm for cont
+Ni0 is starting nvm for intermittent
+ N1 V1 is middle state for intermittent
+N, V, c is checkpoint at middle state of intermittent
+ Nend, Vend is final state for intermittent, not used, solely to fill out the type
+ V1 isn't used anywhere it's just to fill out the type
+ N2, V2 is final state for intermittent, once again solely to fill out the type*)
+Inductive current_init_pt: nvmem -> vmem -> command -> nvmem -> nvmem -> nvmem -> Prop:=
+  valid_mem: forall {N Ni0 N1 Nc0 Nend: nvmem}
+                  {V V1 Vend: vmem}
+                  {c crem: command}
+                  {W : the_write_stuff}
+                  {O: obseq}
+                  {w: warvars}
+                  (T: trace_c (Ni0, V, c) (Nend, Vend, crem) O W),
+    crem = skip \/ (exists(w: warvars) (crem2: command), crem = ((incheckpoint w);;crem2)) ->
+                 subseq (getdomain Nc0) (getdomain N1) 
+                  -> not (checkpoint \in O) (*checks checkpoint T ends on is nearest checkpoint*)
+                 -> (forall(l: loc),
+                      not((getmap N1) l = (getmap Nc0) l)
+                      -> (l \in (getfstwt W)) \/ (l \in (getdomain N)))
+                 -> current_init_pt N V c Ni0 N1 Nc0.
+(*Definition 6*)
+(*concern: Typo in paper, N0, V0 is left out of invocation of Def 4*)
+(*(N0, V0, c0) is checkpoint state at time c1
+N1 V c is intermittent state
+N2 V c is continuous state starting from same state as checkpoint
+concern: using context instead of cconf
+ *)
+(*took out equality premises and built them into the types*)
+Check same_pt.
+Inductive same_config: iconf -> context -> Prop :=
+  SameConfig: forall(N0 N1 N2: nvmem)
+                (V0 V: vmem)
+                (c0 c: command),
+                same_pt N0 V0 c0 c N1 N2 -> (*nvms are extensionally the same by same_pt
+                                          vms and cs are intensionally the same by types*)
+                same_config ((N0, V0, c0), N1, V, c) (N2, V, c).
+
+Close Scope type_scope.
