semantics/proofs_sc.v
@@ -1,0 +1,41 @@
+Set Warnings "-notation-overridden,-parsing".
+From Coq Require Import Bool.Bool Init.Nat Arith.Arith Arith.EqNat
+     Init.Datatypes Strings.String Program Logic.FunctionalExtensionality.
+Require Export Coq.Strings.String.
+From mathcomp Require Import ssreflect ssrfun ssrbool eqtype seq fintype ssrnat ssrfun.
+From TLC Require Import LibTactics LibLogic.
+From Semantics Require Export programs semantics algorithms lemmas_1
+     lemmas_0 proofs_0. (*shouldn't have to import both of these*)
+
+Inductive all_diff_in_fww: nvmem -> vmem -> command -> nvmem -> Prop :=
+  Diff_in_FWw: forall{N1 V1 c1 N2 V2 c2 N1c O W} (T: trace_cs (N1, V1, c1) (N2, V2, c2) O W),
+    checkpoint \notin O -> (*c2 is nearest checkpoint or termination*)
+  (*  (getdomain N1) = (getdomain N1c) -> alternatively
+                                       could check N2 domain as well instead of this
+ not even clear why i need the domains                                    
+   *)
+( forall(l: loc ), ((getmap N1) l <> (getmap N1c) l) -> (l \in getfstwt W))
+-> all_diff_in_fww N1 V1 c1 N1c.
+  Lemma same_com_hc {N N1 V c Nend2 V1 c1 O W}:
+  all_diff_in_fww N V c N1 ->
+  cceval_w (N1, V, c) O (Nend2, V1, c1) W -> (*use that W2 must be a subset of W*)
+  checkpoint \notin O ->
+  exists (Nend1: nvmem), cceval_w (N, V, c) O (Nend1, V1, c1) W
+                             /\ all_diff_in_fww Nend1 V1 c1 Nend2.
+
+
+Admitted.
+
+  Lemma same_com_help {N N1 V c Nend2 Vend cend O W}:
+  all_diff_in_fww N V c N1 ->
+  trace_cs (N1, V, c) (Nend2, Vend, cend) O W ->
+  checkpoint \notin O ->
+  exists (Nend1: nvmem), trace_cs (N, V, c) (Nend1, Vend, cend) O W
+  .
+    intros. move: N H.
+    dependent induction H0; intros N Hdiff.
+    + exists N. apply CsTrace_Empty.
+    + move: (same_com_hc Hdiff H H1) => [Nend1 [done blah] ].
+      exists Nend1. by apply CsTrace_Single.
+    + suffices: 
+Admitted.
